Refine queries for protocol drivers
Co-authored-by: Copilot <223556219+Copilot@users.noreply.github.com>

common/Common.ConnectionStateQuery.fst
@@ -5,7 +5,42 @@ module Common.ConnectionStateQuery
 open Pulse.Lib.Pervasives
 
 module CPI = Common.ProtocolImplementation
+module SZ = FStar.SizeT
 module TCP = Common.TCP
+module U8 = FStar.UInt8
+
+type next_action
+  (local_event:Type0)
+  (external_action:Type0)
+  =
+  | NextNeedInput
+  | NextLocal: ev:local_event -> next_action local_event external_action
+  | NextExternal: action:external_action -> next_action local_event external_action
+  | NextDone
+  | NextFailed
+
+let next_action_correct
+  (#impl:Type0)
+  (#state:Type0)
+  (#local_event:Type0)
+  (#external_action:Type0)
+  (#query:Type0)
+  (network_enabled:impl -> query -> state -> prop)
+  (local_enabled:impl -> query -> state -> local_event -> prop)
+  (external_enabled:impl -> query -> state -> external_action -> prop)
+  (done_enabled:impl -> query -> state -> prop)
+  (failed_enabled:impl -> query -> state -> prop)
+  (i:impl)
+  (q:query)
+  (st:state)
+  (action:next_action local_event external_action)
+  : prop =
+  match action with
+  | NextNeedInput -> network_enabled i q st
+  | NextLocal ev -> local_enabled i q st ev
+  | NextExternal ext -> external_enabled i q st ext
+  | NextDone -> done_enabled i q st
+  | NextFailed -> failed_enabled i q st
 
 noextract
 class connection_state_query
@@ -15,7 +50,7 @@ class connection_state_query
   (local_event:Type0)
   (local_output:Type0)
   (query:Type0)
-  (action:Type0)
+  (external_action:Type0)
   (protocol:CPI.protocol_implementation
     impl
     state
@@ -39,15 +74,125 @@ class connection_state_query
     query ->
     csq_frame ->
     state ->
-    action ->
+    next_action local_event external_action ->
     slprop;
 
-  csq_action_sound:
+  csq_network_enabled:
     impl ->
     query ->
     state ->
-    action ->
     prop;
+
+  csq_local_enabled:
+    impl ->
+    query ->
+    state ->
+    local_event ->
+    prop;
+
+  csq_external_enabled:
+    impl ->
+    query ->
+    state ->
+    external_action ->
+    prop;
+
+  csq_done_enabled:
+    impl ->
+    query ->
+    state ->
+    prop;
+
+  csq_failed_enabled:
+    impl ->
+    query ->
+    state ->
+    prop;
+
+  csq_network_frame_pre:
+    impl ->
+    query ->
+    protocol.CPI.pi_network_frame ->
+    array U8.t ->
+    SZ.t ->
+    array U8.t ->
+    SZ.t ->
+    TCP.bytes ->
+    TCP.bytes ->
+    slprop;
+
+  csq_prepare_network:
+    i:impl ->
+    q:query ->
+    frame:protocol.CPI.pi_network_frame ->
+    input:array U8.t ->
+    input_len:SZ.t ->
+    out:array U8.t ->
+    out_len:SZ.t ->
+    st:Ghost.erased state ->
+    input_contents:Ghost.erased TCP.bytes ->
+    old_out:Ghost.erased TCP.bytes ->
+      stt unit
+        (csq_network_frame_pre
+          i
+          q
+          frame
+          input
+          input_len
+          out
+          out_len
+          (Ghost.reveal input_contents)
+          (Ghost.reveal old_out) **
+         pure (csq_network_enabled i q (Ghost.reveal st)))
+        (fun _ ->
+          protocol.CPI.pi_network_frame_pre
+            frame
+            input
+            input_len
+            out
+            out_len
+            (Ghost.reveal input_contents)
+            (Ghost.reveal old_out));
+
+  csq_local_frame_pre:
+    impl ->
+    query ->
+    local_event ->
+    protocol.CPI.pi_local_frame ->
+    state ->
+    array U8.t ->
+    SZ.t ->
+    TCP.bytes ->
+    slprop;
+
+  csq_prepare_local:
+    i:impl ->
+    q:query ->
+    ev:local_event ->
+    frame:protocol.CPI.pi_local_frame ->
+    out:array U8.t ->
+    out_len:SZ.t ->
+    st:Ghost.erased state ->
+    old_out:Ghost.erased TCP.bytes ->
+      stt unit
+        (csq_local_frame_pre
+          i
+          q
+          ev
+          frame
+          (Ghost.reveal st)
+          out
+          out_len
+          (Ghost.reveal old_out) **
+         pure (csq_local_enabled i q (Ghost.reveal st) ev))
+        (fun _ ->
+          protocol.CPI.pi_local_frame_pre
+            ev
+            frame
+            (Ghost.reveal st)
+            out
+            out_len
+            (Ghost.reveal old_out));
 
   csq_next_action:
     i:impl ->
@@ -56,7 +201,7 @@ class connection_state_query
     received:Ghost.erased TCP.bytes ->
     sent:Ghost.erased TCP.bytes ->
     st:Ghost.erased state ->
-      stt action
+      stt (next_action local_event external_action)
         (protocol.CPI.pi_invariant
           i
           (Ghost.reveal received)
@@ -79,5 +224,14 @@ class connection_state_query
             frame
             (Ghost.reveal st)
             action **
-          pure (csq_action_sound i q (Ghost.reveal st) action));
+          pure (next_action_correct
+            csq_network_enabled
+            csq_local_enabled
+            csq_external_enabled
+            csq_done_enabled
+            csq_failed_enabled
+            i
+            q
+            (Ghost.reveal st)
+            action));
 }
